EquivalenceC.v
@@ -1,0 +1,40 @@
+Require Import SessionTypesC.
+
+Module EqC.
+Import StyC.
+
+Inductive sequiv_gen sequiv : Sty -> Sty -> Prop :=
+| sequiv_gen_end : sequiv_gen sequiv unit unit
+| sequiv_gen_send : forall B S S',
+    sequiv S S' ->
+    sequiv_gen sequiv (send B S) (send B S')
+| sequiv_gen_recv : forall B S S',
+    sequiv S S' ->
+    sequiv_gen sequiv (recv B S) (recv B S')
+| sequiv_gen_echoice : forall S1 S2 S1' S2',
+    sequiv S1 S1' ->
+    sequiv S2 S2' ->
+    sequiv_gen sequiv (echoice S1 S2) (echoice S1' S2')
+| sequiv_gen_ichoice : forall S1 S2 S1' S2',
+    sequiv S1 S1' ->
+    sequiv S2 S2' ->
+    sequiv_gen sequiv (ichoice S1 S2) (ichoice S1' S2')
+| sequiv_gen_mu1 : forall XS S S',
+    sequiv (substc XS S) S' ->
+    sequiv_gen sequiv (mu XS S) S'
+| sequiv_gen_mu2 : forall XS S S',
+    sequiv S (substc XS S') ->
+    sequiv_gen sequiv S (mu XS S')
+.
+Hint Constructors sequiv_gen.
+
+CoInductive sequiv : Sty -> Sty -> Prop :=
+| sequiv_fold : forall S S', sequiv_gen sequiv S S' -> sequiv S S'.
+Hint Constructors sequiv.
+
+Lemma sequiv_coind : forall R,
+  (forall S S', R S S' -> sequiv_gen R S S')
+  -> (forall S S', R S S' -> sequiv S S').
+Proof. cofix CIH. intros R H S S' HR. apply H in HR. inversion HR; eauto. Qed.
+
+End EqC.
